ocaml/coq_driver/test/tzel_wots.mli
@@ -3,6 +3,10 @@ type felt = bytes
 
 val hash3 : felt -> felt -> felt -> felt
 
+val hash5 : felt -> felt -> felt -> felt -> felt -> felt
+
+val commit : felt -> felt -> felt -> felt -> felt -> felt
+
 val pack_adrs_chain : int -> int -> int -> felt
 
 val xmss_chain_step : felt -> felt -> int -> int -> int -> felt
